working on composition

theories/prob_eff_lang/probblaze/examples/DH_KE/new_composition.v
@@ -151,18 +151,21 @@ Section new_comp_verification.
                   BREL v1 ((λ: "m", do: leakauth1 (Send "m")), (λ: "m", do: leakauth1 (Recv "m")))%V (λ: "m", do: keyleak1 "m")%V ≤ v2 ((λ: "m", do: leakauth2 (Send "m")), (λ: "m", do: leakauth2 (Recv "m")))%V (λ: "m", do: keyleak2 "m")%V <| (iLblSig_to_iLblThy (envsec_row keyleak1 keyleak2 leakauth1 leakauth2 )) ++ (iLblSig_to_iLblThy L) |> {{ (λ w1 w2, 𝟙%T w1 w2)}}}}.
      Proof.
      Admitted. *)
-  
-  Definition bla : val :=
+
+  Definition bla0 : val :=
+    (λ: "f", ((λ: "f", F_AUTH (DH_SIM (F_KE "f")))%V ||ᵣ F_OAUTH) (CHAN "f")). 
+
+  Definition bla1 : val :=
     (λ: "f", ((λ: "f", (λ: "f", F_AUTH (DH_SIM "f"))%V (F_KE "f"))%V ||ᵣ F_OAUTH) (CHAN "f")). 
 
   Definition bla2 : val :=
-    (λ: "f", (λ: "f" "rF" "rH", (λ: "f", F_AUTH (DH_SIM "f"))%V (λ: "rG", (F_KE ||ᵣ F_OAUTH) "f" "rH" "rG") "rF") (CHAN "f")).
+    (λ: "f", (λ: "f" "rF" "rH", (λ: "f", F_AUTH (DH_SIM "f"))%V (λ: "rG", (F_KE ||ᵣ F_OAUTH)%V "f" "rH" "rG") "rF") (CHAN "f")).
 
   Definition bla3 : val :=
-    (λ: "f" "rF" "rH", (λ: "f", F_AUTH (DH_SIM "f")) (λ: "rG", (λ: "f", (F_KE_L ||ᵣ F_OAUTH) (CHAN "f")) "f" "rH" "rG") "rF"). 
+    (λ: "f" "rF" "rH", (λ: "f", F_AUTH (DH_SIM "f"))%V (λ: "rG", (λ: "f", (F_KE ||ᵣ F_OAUTH)%V (CHAN "f")) "f" "rH" "rG") "rF"). 
 
   Lemma REAL_CHAN_DH_RAND_bla : 
-    ⊢ sem_val_typed REAL_CHAN_DH_RAND bla (∀ᵣ θ__L ,(∀ᵣ θₕ, (((⊤ × (sem_ty_sum 𝟙 𝟙)) -{ θₕ }-> 𝟙) × ((sem_ty_sum 𝟙 𝟙) -{ θₕ }-> (Option  ⊤))) 
+    ⊢ sem_val_typed REAL_CHAN_DH_RAND bla0 (∀ᵣ θ__L ,(∀ᵣ θₕ, (((⊤ × (sem_ty_sum 𝟙 𝟙)) -{ θₕ }-> 𝟙) × ((sem_ty_sum 𝟙 𝟙) -{ θₕ }-> (Option  ⊤))) 
                                                                    -{ sem_row_union  θₕ θ__L }-> 𝟙)
                                                              ⊸ (∀ᵣ θ1,∀ᵣ θ2, (((⊤ × (𝟙 + 𝟙)) -{ θ1 }-> 𝟙) 
                                                                                  × ((𝟙 + 𝟙) -{ θ1 }-> Option ⊤)) 
@@ -173,14 +176,33 @@ Section new_comp_verification.
     - admit.
     - admit.
     - iIntros (θ). iApply parallel_comp_right. 
-      + iApply func_comp_assoc. iApply F_AUTH_C_DH_rand_FAUTH_DH_SIM_F_KE; try done.
+      + iApply F_AUTH_C_DH_rand_FAUTH_DH_SIM_F_KE; try done.
       + admit.
     - admit.
   Admitted. 
         
-
-  Lemma bla_bla2 :
-    ⊢ sem_val_typed bla bla2 (∀ᵣ θ__L ,(∀ᵣ θₕ, (((⊤ × (sem_ty_sum 𝟙 𝟙)) -{ θₕ }-> 𝟙) × ((sem_ty_sum 𝟙 𝟙) -{ θₕ }-> (Option  ⊤))) 
+  Lemma bla0_bla1 : 
+    ⊢ sem_val_typed bla0 bla1 (∀ᵣ θ__L ,(∀ᵣ θₕ, (((⊤ × (sem_ty_sum 𝟙 𝟙)) -{ θₕ }-> 𝟙) × ((sem_ty_sum 𝟙 𝟙) -{ θₕ }-> (Option  ⊤))) 
+                                                                   -{ sem_row_union  θₕ θ__L }-> 𝟙)
+                                                             ⊸ (∀ᵣ θ1,∀ᵣ θ2, (((⊤ × (𝟙 + 𝟙)) -{ θ1 }-> 𝟙) 
+                                                                                 × ((𝟙 + 𝟙) -{ θ1 }-> Option ⊤)) 
+                                                                                 ⊸ (((⊤ × (𝟙 + 𝟙)) -{ θ2 }-> 𝟙) 
+                                                                                 × ((𝟙 + 𝟙) -{ θ2 }-> Option ⊤)) -{ sem_row_union θ1 (sem_row_union θ2 θ__L) }-∘ 𝟙))%T.
+  Proof.
+    iApply func_comp_left.
+    - admit.
+    - admit.
+    - iIntros (θ). iApply parallel_comp_right.
+      + unfold τ__F. iApply func_comp_assoc.
+        * admit.
+        * admit.
+        * admit.
+      + admit.
+    - admit.
+  Admitted. 
+        
+  Lemma bla1_bla2 :
+    ⊢ sem_val_typed bla1 bla2 (∀ᵣ θ__L ,(∀ᵣ θₕ, (((⊤ × (sem_ty_sum 𝟙 𝟙)) -{ θₕ }-> 𝟙) × ((sem_ty_sum 𝟙 𝟙) -{ θₕ }-> (Option  ⊤))) 
                                                                    -{ sem_row_union  θₕ θ__L }-> 𝟙)
                                                              ⊸ (∀ᵣ θ1,∀ᵣ θ2, (((⊤ × (𝟙 + 𝟙)) -{ θ1 }-> 𝟙) 
                                                                                  × ((𝟙 + 𝟙) -{ θ1 }-> Option ⊤)) 
@@ -188,17 +210,30 @@ Section new_comp_verification.
                                                                                  × ((𝟙 + 𝟙) -{ θ2 }-> Option ⊤)) -{ sem_row_union θ1 (sem_row_union θ2 θ__L) }-∘ 𝟙))%T.
   Proof.
     (* All admits are well-typedness *)
-    unfold bla, bla2.
     iApply func_comp_left.
-    - admit.
-    - admit.
-    - iIntros (θ). iApply parallel_comp_right. func_comp_parallel_comp_assoc.
+    - admit.                    (* closed expr *)
+    - admit.                    (* closed expr *)
+    - iIntros (θ). iApply func_comp_parallel_comp_assoc.
       + admit.
       + admit.
       + admit.
     - admit.
   Admitted.
   
-  Lemma bla2_bla3 : val
+  Lemma bla2_bla3 :
+    ⊢ sem_val_typed bla2 bla3 (∀ᵣ θ__L ,(∀ᵣ θₕ, (((⊤ × (sem_ty_sum 𝟙 𝟙)) -{ θₕ }-> 𝟙) × ((sem_ty_sum 𝟙 𝟙) -{ θₕ }-> (Option  ⊤))) 
+                                              -{ sem_row_union  θₕ θ__L }-> 𝟙)
+                                        ⊸ (∀ᵣ θ1,∀ᵣ θ2, (((⊤ × (𝟙 + 𝟙)) -{ θ1 }-> 𝟙) 
+                                                           × ((𝟙 + 𝟙) -{ θ1 }-> Option ⊤)) 
+                                                          ⊸ (((⊤ × (𝟙 + 𝟙)) -{ θ2 }-> 𝟙) 
+                                                               × ((𝟙 + 𝟙) -{ θ2 }-> Option ⊤)) -{ sem_row_union θ1 (sem_row_union θ2 θ__L) }-∘ 𝟙))%T.
+  Proof. 
+    unfold bla2, bla3.
+    iApply functionality_comp_func_comp_assoc.
+  Qed. 
+
+  Lemma 
+
+                      
 
 End new_comp_verification.
